doc/tutorial/code/solutions/Ex12b.RPC.fst
@@ -1,18 +1,24 @@
 module Ex12b.RPC
 
-open FStar.HyperStack.ST
-open FStar.HyperStack.All
-open FStar.Seq
-open FStar.Monotonic.Seq
-open FStar.HyperHeap
-open FStar.HyperStack
-open FStar.Monotonic.RRef
+(* open FStar.HyperStack.ST *)
+(* open FStar.Seq *)
+(* open FStar.Monotonic.Seq *)
+(* open FStar.HyperHeap *)
+(* open FStar.HyperStack *)
+(* open FStar.Monotonic.RRef *)
 
-open FStar.String
 open FStar.IO
 
+open Preorder
+open Heapx
+open STx
+open MRefx
 
-let init_print = print_string "\ninitializing...\n\n"
+open FStar.List.Tot
+open FStar.String
+
+
+let init_print = debug_print_string "\ninitializing...\n\n"
 
 open Platform.Bytes
 open Ex12.SHA1
@@ -25,20 +31,18 @@ module Formatting = Ex12b2.Format
 (* some basic, untrusted network controlled by the adversary *)
 
 
-val msg_buffer: FStar.HyperStack.ref message
-let msg_buffer = FStar.HyperStack.ST.ralloc root (empty_bytes)
+val msg_buffer: ref message
+let msg_buffer = alloc _ (empty_bytes)
 
 // BEGIN: Network
-private val send: message -> ML unit
-private val recv: (message -> ML unit) -> ML unit
+private val send: message -> St unit
+private val recv: (message -> St unit) -> St unit
 // END: Network
 
 let send m = 
-  recall msg_buffer;
   msg_buffer := m
 
 let rec recv call = 
-  recall msg_buffer;
   if length !msg_buffer > 0
   then (
     let msg = !msg_buffer in
@@ -54,12 +58,31 @@ type log_entry =
   | Response: string -> string -> log_entry
   
 
-private type log_t (r:rid) = Monotonic.Seq.log_t r log_entry
-let log:log_t root = alloc_mref_seq #log_entry root createEmpty
+(* private type log_t (r:rid) = Monotonic.Seq.log_t r log_entry *)
+(* let log:log_t root = alloc_mref_seq #log_entry root createEmpty *)
+
+let subset' (#a:eqtype) (l1:list a) (l2:list a)
+  = (forall x. x `mem` l1 ==> x `mem` l2)
+let subset (#a:eqtype) : Tot (preorder (list a)) = subset'
+
+type lref = mref (list log_entry) subset
+
+private let log : lref = alloc (subset #log_entry) []
+
+let add_to_log (r:lref) (v:log_entry) :
+      ST unit (requires (fun _ -> True))
+              (ensures (fun _ _ h -> v `mem` (sel h r))) =
+  r := (v :: !r)
 
 // BEGIN: RpcPredicates
-type pRequest s = exists n. witnessed (at_least n (Request s) log)
-type pResponse s t = exists n. witnessed (at_least n (Response s t) log)
+
+let req s : Tot (p:(list log_entry -> Type0){Preorder.stable p subset})
+  = fun xs -> mem (Request s) xs
+let resp s t : Tot (p:(list log_entry -> Type0){Preorder.stable p subset})
+  = fun xs -> mem (Response s t) xs
+
+type pRequest s = token log (req s)
+type pResponse s t = token log (resp s t)
 // END: RpcPredicates
 
 (* the meaning of MACs, as used in RPC *)
@@ -76,69 +99,76 @@ let k = ignore (debug_print_string "generating shared key...\n");
 
 
 
-val client_send : s:string16 -> ML (u:unit)
+val client_send : s:string16 -> St unit
 let client_send (s:string16) =
-  m_recall log;
   ignore (debug_print_string "\nclient send:");
   ignore (debug_print_string s);
-  write_at_end log (Request s);
+  add_to_log log (Request s);
+  witness log (req s);
   
   assert(reqresp (Formatting.request s)); (* this works *)
   assert(key_prop k == reqresp);          (* this also works *)
   assert(key_prop k (Formatting.request s) == reqresp (Formatting.request s));
   (*assert(key_prop k (Formatting.request s)); -- this fails *)
-  m_recall log;
   send ( (utf8 s) @| (mac k (Formatting.request s)))
 
 
-val client_recv : string16 -> ML unit
+val client_recv : string16 -> St unit
 let client_recv (s:string16) =
   recv (fun msg ->
-    if length msg < macsize then failwith "Too short"
+    if length msg < macsize then ignore (debug_print_string "Too short")
     else
       let (v, m') = split msg (length msg - macsize) in
       let t = iutf8 v in
       if verify k (Formatting.response s t) m'
       then (
         assert (pResponse s t);
+        recall log (resp s t);
+        let xs = !log in
+        assert (Response s t `mem` xs);
         ignore (debug_print_string "\nclient verified:");
         ignore (debug_print_string t) ))
 
-
 // BEGIN: RpcProtocol
-val client : string16 -> ML unit
+val client : string16 -> St unit
 let client (s:string16) =
   client_send s;
   client_recv s
 
-val server : unit -> ML unit
+val server : unit -> St unit
 let server () =
   recv (fun msg ->
-    if length msg < macsize then failwith "Too short"
+    if length msg < macsize then ignore (debug_print_string "Too short")
     else
       let (v,m) = split msg (length msg - macsize) in
-      if length v > 65535 then failwith "Too long"
+      if length v > 65535 then ignore (debug_print_string "Too long")
       else
         let s = iutf8 v in
         if verify k (Formatting.request s) m
         then
-          ( 
+          (
             assert (pRequest s);
+            recall log (req s);
+            let xs = !log in
+            assert (Request s `mem` xs);
             ignore (debug_print_string "\nserver verified:");
             ignore (debug_print_string s);
             let t = "42" in
-            write_at_end log (Response s t);
+            add_to_log log (Response s t);
+            witness log (resp s t);
             ignore (debug_print_string "\nserver sent:");
             ignore (debug_print_string t);
-            send ( (utf8 t) @| (mac k (Formatting.response s t))))
-        else failwith "Invalid MAC" )
+            send ( (utf8 t) @| (mac k (Formatting.response s t)))
+            )
+        else ignore (debug_print_string "Invalid MAC" ))
 // END: RpcProtocol
 
-private val test : unit -> ML unit
+private val test : unit -> St unit
 let test () =
   let query = "4 + 2" in
-  if length (utf8 query) > 65535 then failwith "Too long"
+  if length (utf8 query) > 65535 then ignore (debug_print_string "Too long")
   else
+    let query : string16 = query in
     client_send query;
     server();
     client_recv query;
